MemoNat/DArray.lean
@@ -19,6 +19,20 @@ theorem Any.congr.{u} {a₁ a₂ : Any}  (h : a₁ = a₂) {α : Sort u} {h₁ :
     {h₂ : a₂.Sort = α} :
     h₁ ▸ a₁.val = h₂ ▸ a₂.val := by induction h; rfl
 
+theorem Any.rw.{u} {a₁ a₂ : Any}  (h : a₁ = a₂) {α : Sort u} {h₁ : a₁.Sort = α} :
+    h₁ ▸ a₁.val = (h ▸ h₁) ▸ a₂.val := by induction h; rfl
+
+theorem Any.eq_rec_val.{u} {α : Sort u} {a : Any} (h : a.Sort = α) (x : α) (eq : a = Any.mk x) :
+    h ▸ a.val = x := by cases eq; rfl
+
+@[simp]
+theorem Any.mk_eq_rec.{u₁,u₂} {β : Sort u₁} {x y : β} {P : β → Sort u₂} (h : x = y) (a : P x):
+    Any.mk (h ▸ a) = Any.mk a := by cases h; rfl
+
+@[simp]
+theorem Any.mk_eq_rec'.{u}  {α β : Sort u} (h : α = β) (a : α) :
+    Any.mk (h ▸ a) = Any.mk a := @Any.mk_eq_rec _ α β (fun x => x) h a
+
 --  (_ : Any.Sort (Array.get (Array.push { arr := a, types := types }.arr (Any.mk x)) i) = C i.val) ▸
     -- Any.val (Array.push a (Any.mk x))
 
@@ -28,12 +42,12 @@ structure DArray.{u} (C : Nat → Type u) : Type (u+1):=
 
 namespace DArray
 
-protected def empty {C} (cap : Nat) : DArray C :=
+def mkEmpty {C} (cap : Nat) : DArray C :=
   ⟨ Array.mkEmpty cap, λ i => Fin.elim0 i⟩
 
 def size {C} (a : DArray C) := a.arr.size
 
-protected def push {C} (a : DArray C) (x : C a.size) : DArray C :=
+def push {C} (a : DArray C) (x : C a.size) : DArray C :=
   ⟨ a.arr.push (Any.mk x),
    by 
     cases a with | _ a types =>
@@ -52,15 +66,14 @@ protected def push {C} (a : DArray C) (x : C a.size) : DArray C :=
       rfl
   ⟩
 
-protected theorem size_push {C} (a : DArray C) (x : C a.size) : (a.push x).size = a.size + 1 :=
+theorem size_push {C} (a : DArray C) (x : C a.size) : (a.push x).size = a.size + 1 :=
   Array.size_push _ _
 
-protected def get.{u} {C : Nat → Type u} (a : DArray C) (i : Fin a.size) : C i :=
+def get.{u} {C : Nat → Type u} (a : DArray C) (i : Fin a.size) : C i :=
   let x : Any := Array.get a.arr i
   a.types i ▸ x.val
 
-
-protected theorem get_push {C} (a : DArray C) (x : C a.size) (i : Fin (a.push x).size) :
+theorem get_push {C} (a : DArray C) (x : C a.size) (i : Fin (a.push x).size) :
     (a.push x).get i =
       if h : i < a.size
       then a.get ⟨i, h⟩
@@ -69,30 +82,14 @@ protected theorem get_push {C} (a : DArray C) (x : C a.size) (i : Fin (a.push x)
           (Nat.le_of_not_lt h)
           (Nat.le_of_lt_succ (by simpa [a.size_push x] using i.isLt))
         (this ▸ x : C i) := by
-  split 
-  case inl hi2 =>
-    rcases a with ⟨a, types⟩ 
-    apply Any.congr
-    dsimp
-    unfold DArray.push
-    rw [Array.get_push ]
-    dsimp
-    dsimp [DArray.size] at hi2
-    simp [hi2]
+  apply (Any.rw (Array.get_push a.arr (Any.mk x) i.val i.isLt)).trans
+  apply Any.eq_rec_val
+  unfold DArray.size
+  split
+  case inl _ =>
+    simp only [get, Array.get, Any.mk_eq_rec']
+    rfl
   case inr hi2 =>
-    have : size a = i := Nat.le_antisymm
-      (Nat.le_of_not_lt hi2)
-      (Nat.le_of_lt_succ (by simpa [a.size_push x] using i.isLt))
-    rcases a with ⟨a, types⟩ 
-    dsimp [DArray.get, DArray.push]
-    sorry
-    
-
-
-    
-
-  -- rw [ SArray.get_push a.1 (Any.mk x) i hi ]
-  sorry
-  
+    simp only [get, Array.get, Any.mk_eq_rec', DArray.size, Any.mk_eq_rec ]
 
 end DArray
